---
title: Multiplicativity of Ramanujan τ function
feed: [[Multiplicativity of Ramanujan τ function]]
date: 11-05-2022
permalink: /credits
format: list
---
*first part is trivial also, given that it is a modular form.*

Define $F_p(\tau)=p^{11}\Delta(p\tau)+\frac 1 p \sum_{k=0}^{p-1}\Delta\left(\frac{\tau+k}{p}\right)$.
Since the [[modular discriminant]] $\Delta(\tau)$ is a modular form of weight 12, $\Delta(\tau+1)=\Delta(\tau)$. Hence, $\Delta(p(\tau+1))=\Delta(p\tau+p)=\Delta(p\tau)$. Also, $\Delta\left(\frac{\tau+p}{p}\right)=\Delta(\tau+1)=\Delta(\tau)$. Hence, the two terms in $F_p(\tau+1)$ are same as those in $F_p(\tau)$. Thus, $F_p(\tau+1)=F_p(\tau)$.



Wrong: *I don't understand the definition. Since its a modular form, why is it not just $p^{11}(p+1)\Delta(\tau)$? If I'm right, I don't need the previous part of the problem. **need ad-bc=1!*** 
$F_p(\tau+1)=F_p(\tau)$ since the [[modular discriminant]] $\Delta(\tau)$ is a modular form of weight 12 $\rightarrow$ 
$\Delta(p\tau)=\Delta(\tau), \Delta\left(\frac{\tau+k}{p}\right)=\Delta(\tau)$. Or, it just follows from the above question.


reduced residue system
euler totient function



![[apostol.pdf#page=102]]